src/MemInjProps.v
@@ -1,0 +1,20 @@
+Require Import compcert.common.Values.
+Require Import compcert.common.Memory.
+Require Import compcert.common.Globalenvs.
+
+Local Open Scope Z_scope.
+
+
+(* nothing is moved around within blocks *)
+Definition same_offsets (mi : meminj) : Prop :=
+  forall b b' delta,
+    mi b = Some (b',delta) ->
+    delta = 0.
+
+(* globals aren't moved around *)
+Definition globals_inj_same {F V} (ge : Genv.t F V) (mi : meminj) : Prop :=
+  forall b f v,
+    (Genv.find_funct_ptr ge b = Some f \/
+    Genv.find_var_info ge b = Some v) ->
+    mi b = Some (b,0).
+
